Ground_PDDL_Exec_Imp/Ground_PDDL_Plan_Reduction.thy
@@ -1,0 +1,20 @@
+theory Ground_PDDL_Plan_Reduction
+  imports Ground_PDDL_Plan_Defs Ground_PDDL_Problem_Reduction
+begin
+
+context valid_ground_plan
+begin
+sublocale red_corr: tp_nta_reduction_correctness' init_spec goal_spec 
+  at_start_spec at_end_spec over_all_spec
+  lower_spec upper_spec pre_spec adds_spec dels_spec
+  0 
+  props_spec actions_spec plan_imp  
+  act_to_name_spec prop_to_name_spec
+  apply unfold_locales
+  using temp_plan_valid apply simp
+  using temp_plan_no_self_overlap apply blast
+  using temp_plan_actions_in_actions apply blast
+  done
+end
+
+end
